Defined step up to primitives. Added examples.
We have defined plus and provided some examples of stepping through a
simple program. We still need to work on defining evaluation contexts
however, so we can't evaluate more complex examples (as demonstrated by
the admit towards the end.)

Atomicity.v
@@ -9,8 +9,8 @@
  Require Import SfLib.
 
 Inductive conflict : Type :=
-  | None : conflict
-  | Race : conflict.
+  | CNone : conflict
+  | CRace : conflict.
 
 (* Inductive id : Type :=
   | Id : nat -> id. *)
@@ -22,66 +22,168 @@ end.
 Eval simpl in id_eq (Id 5) (Id 6).
 Eval simpl in id_eq (Id 5) (Id 5).
 
-Inductive value : Type :=
-  | VConst   : nat -> value
-  | VSyncLoc : nat -> value
-  | VFunction: nat -> list id -> value.
+Inductive primitive : Type :=
+  | Assert  : primitive
+  | Plus    : primitive
+  | NewLock : primitive
+  | Acquire : primitive
+  | Release : primitive.
 
 Inductive exp : Type :=
-  | EValue : value -> exp
-  | EId    : id -> conflict -> exp
-  | EAssgn : id -> conflict -> exp -> exp
-  | ESeq   : exp -> exp -> exp
-  | EPrim  : (list value -> value) -> list exp -> exp
-  | ECall  : exp -> list exp -> list exp -> exp
-  | EIf    : exp -> exp -> exp -> exp
-  | EWhile : exp -> exp -> exp
-  | ELet   : id -> exp -> exp -> exp
-  | EFork  : exp -> exp
-  | EAtomic: exp -> exp
+  | EConst    : nat -> exp
+  | ESyncLoc  : id -> exp
+  | EFunction : list id -> exp -> exp
+  | EValue    : exp -> exp
+  | EId       : id -> conflict -> exp
+  | EAssgn    : id -> conflict -> exp -> exp
+  | ESeq      : exp -> exp -> exp
+  | EPrim     : primitive -> list exp -> exp
+  | ECall     : exp -> list exp -> list exp -> exp
+  | EIf       : exp -> exp -> exp -> exp
+  | EWhile    : exp -> exp -> exp
+  | ELet      : id -> exp -> exp -> exp
+  | EFork     : exp -> exp
+  | EAtomic   : exp -> exp
   | EInAtomic : exp -> exp.
 
+Inductive value : exp -> Prop :=
+  | VConst   : forall n, value (EConst n)
+  | VSyncLoc : forall id, value (ESyncLoc id)
+  | VFunction: forall lids exp, value (EFunction lids exp).
+
+Inductive values : list exp -> Prop :=
+  | VEmpty : values []
+  | VList : forall a b, value a -> values b -> values (a::b).
+
+Inductive thread : Type :=
+  | TExpr : exp -> thread
+  | Wrong : thread.
+
+
+
 Notation "x '%' b '::=' n" := (EAssgn x b n) (at level 60).
+Notation "x '%%' b" := (EId x b) (at level 60).
 Notation "a ';' b" := (ESeq a b) (at level 60).
+Notation "a 'p+' b" := (EPrim Plus [a, (EConst b)]) (at level 60).
 Notation "'IFE' x 'THEN' a 'ELSE' b" := (EIf x a b) (at level 60).
 Notation "'WHILE' a 'DO' b" := (EWhile a b) (at level 60).
 Notation "'LET' a '::=' b 'IN' c" := (ELet a b c) (at level 60).
 Notation "'FORK' a" := (EFork a) (at level 60).
 
 Definition i := (Id 5).
-Definition a := (EId i None).
+Definition a := (EId i CNone).
 Definition b := IFE a 
-                THEN LET i ::= a IN (i % (None) ::= (EValue (VConst 6)) )
+                THEN LET i ::= a IN (i % (CNone) ::= (EConst 6) )
                 ELSE WHILE a DO a.
+Definition p := (EConst 5) p+ 6.
 Print b.
 
-Definition heap_state := id -> nat.
+Inductive heap : Type :=
+| HEmpty : heap
+| HHeap  : forall e, value e -> id -> heap -> heap.
+
+Print heap.
+Example heapa := HEmpty.
+Example heapb := HHeap (EConst 5) (VConst 5) (Id 0) HEmpty.
+
 Definition sync_state := id -> nat.
 
-Definition empty_heap : heap_state :=
+Definition empty_sync : sync_state :=
   fun _ => 0.
 
-Definition empty_sync : heap_state :=
-  fun _ => 0.
+Fixpoint lookup_heap (st : heap) (X:id) : option (sig value) :=
+match st with
+| HHeap a b c d => if (beq_id c X) then Some (exist value a b) else lookup_heap d X
+| HEmpty => None
+end.
 
-Definition update_heap (st : heap_state) (X:id) (n : nat) : heap_state :=
-  fun X' => if beq_id X X' then n else st X'.
+(* Goal (forall y, lookup_heap (HHeap (EConst 3) (VConst 3) (Id 5) HEmpty) (Id 5) <> y). *)
+(* intro. intro. destruct y. simpl in H. inversion H. destruct s. inversion H1. ... *)
+
+
+Definition myheap := HHeap (EConst 5) (VConst 5) (Id 0) HEmpty.
+
+(* Definition lookup_heap (st : heap) (X:id) : option (ex value) := *)
+(* match st with *)
+(* | HEmpty => None *)
+(* | HHeap a b c d => Some (ex_intro value a b) *)
+(* end. *)
 
 Definition update_sync (st : sync_state) (X:id) (n : nat) : sync_state :=
   fun X' => if beq_id X X' then n else st X'.
 
-Inductive thread : Type :=
-  | TExpr : exp -> thread
-  | Wrong : thread.
+Print value.
 
-Inductive step : heap_state -> sync_state -> list thread -> Prop :=
-  | SWhile : forall (e1 e2 : exp) (heap : heap_state) (sync : sync_state) (t t' : list thread), 
+
+(* Definition extract (v : option value) := match v with *)
+(*   | Some a => a *)
+(*   | None   => VConst 0 *)
+(* end. *)
+
+
+Definition I (p : primitive) (vs : list exp) (sync_heap : sync_state) : option ((sig value) * sync_state)  := 
+match p with
+  | Assert  => None
+  | Plus    => match vs with
+                 |  (EConst a)::(EConst b)::[] => 
+                      Some (exist value (EConst (a + b)) (VConst (a+b)), sync_heap)
+                 | _ => None
+               end
+  | NewLock => None
+  | Acquire => None
+  | Release => None
+end.
+
+
+
+Inductive step : heap -> sync_state -> list thread -> Prop :=
+  | SWhile : forall (e1 e2 : exp) (heap : heap) (sync : sync_state) (t t' : list thread), 
               step heap sync (t ++ (TExpr (WHILE e1 DO e2))::t') ->
-              step heap sync (t ++ (TExpr (IFE e1 THEN e2; (WHILE e1 DO e2)  ELSE (EValue (VConst 0))))::t')
+              step heap sync (t ++ (TExpr (IFE e1 THEN e2; (WHILE e1 DO e2)  ELSE (EConst 0)))::t')
   | SIf    : forall (e1 e2 : exp) heap sync t t' v,
-             v <> (VConst 0) -> 
+             value v -> v <> (EConst 0) -> 
              step heap sync (t ++ (TExpr (IFE (EValue v) THEN e1 ELSE e2))::t') ->
              step heap sync (t ++ (TExpr e1)::t')
   | SIfZ   : forall (e1 e2 : exp) heap sync t t',
-             step heap sync (t ++ (TExpr (IFE (EValue (VConst 0)) THEN e1 ELSE e2))::t') ->
-             step heap sync (t ++ (TExpr e2)::t').
+             step heap sync (t ++ (TExpr (IFE (EConst 0) THEN e1 ELSE e2))::t') ->
+             step heap sync (t ++ (TExpr e2)::t')
+  | SLet   : forall x v e (p : value v) heap sync t t',
+             lookup_heap heap x = None ->
+             step heap sync (t ++ (TExpr (LET x ::= v IN e))::t') ->
+             step (HHeap v p x heap) sync (t ++ (TExpr e)::t')
+  | SLookup: forall x c heap sync t t' v p,
+             step heap sync (t ++ (TExpr (x %% c))::t') ->
+             lookup_heap heap x = Some (exist value v p) -> 
+             step heap sync (t ++ (TExpr v)::t')
+  | SAssgn : forall x c v p heap sync t t',
+             value v ->
+             step heap sync (t ++ (TExpr (x % (c) ::= v))::t') ->
+             step (HHeap v p x heap) sync (t ++ (TExpr (EValue v))::t')
+  | SPrim  : forall p (es : list exp) heap sync sync' v' t t' val,
+             I p es sync = Some (exist value v' val, sync') ->
+             step heap sync (t ++ (TExpr (EPrim p es))::t') ->
+             step heap sync' (t ++ (TExpr v')::t')
+  | SWrong : forall p (es : list exp) heap sync sync' t t',
+             I p es sync = None ->
+             step heap sync (t ++ (TExpr (EPrim p es))::t') ->
+             step heap sync' (t ++ (Wrong)::t').
+
+Example Example1 : forall heap sync_state t t', step heap sync_state (t ++ (TExpr ((EConst 1) p+ 2))::t') ->
+  step heap sync_state (t ++ (TExpr (EConst 3))::t').
+  intros heap sync' t t' H. 
+  apply SPrim with (p:=Plus) (es:=[EConst 1, EConst 2]) (val:=VConst 3) (sync:=sync'). 
+  reflexivity.
+  assumption.
+Qed.
+
+Check (EConst 1) p+ 2 p+ 3.
+
+Example Example2 : forall heap sync_state t t', step heap sync_state (t ++ (TExpr (IFE (EConst 2) p+ 3 THEN (EConst 5) ELSE (EConst 6)))::t') ->
+  step heap sync_state (t ++ (TExpr (EConst 5))::t').
+  intros heap sync' t t' H. 
+  apply SIf with (e2:=(EConst 6)) (v:=EConst 5).
+  apply VConst.
+  discriminate.
+  admit.
+Qed.
+
